First-cut proofs with translation EVM-IR to EVM.

src/dafny/refinement/evmir-refinement-general.dfy
@@ -33,18 +33,140 @@ module EVMIRSimulationFull {
     /**
      *  Translate and EVMir program into a EVM program.
      */
-    function method toEVM<S>(p: EVMIRProg): map<nat, EVMProg>
+    function method toEVM<S>(p: EVMIRProg): seq<EVMProg2>
     {
         match p 
-            case Block(i) => map[1 := AInst(i)]
+            case Block(i) => [EVMProg2.AInst(i)]
             case While(c, Block(b)) => 
-                map[
-                    1 := Jumpi(negF(c), 3), 
-                    2 := AInst(b),
-                    3 := Jump(1)
+                [
+                    EVMProg2.Jumpi(negF(c), 3),     // 0
+                    EVMProg2.AInst(b),              // 1
+                    EVMProg2.Jump(-2)               // 2
                 ]
-            case _ => map[]
+            case IfElse(cond, Block(b1), Block(b2)) => 
+                [
+                    EVMProg2.Jumpi(negF(cond), 3),  // 0
+                    EVMProg2.AInst(b1),             // 1
+                    EVMProg2.Jump(2),               // 2
+                    EVMProg2.AInst(b2)              // 3
+                ]
+            case _ =>   //  Cases not covered
+                []
     }
+
+    //  Translation proof (simple)
+    /**
+     *  Single While loop. Assume Unique block in loop body.
+     *
+     *  @returns    The (minimum) number of steps in the EVMIR to simulate n steps in EVM. 
+     */
+    // lemma singleWhileSim<S>(i: EVMInst, cond: S -> bool, n: nat, s: S) returns (k: nat)
+    //      ensures k <= n && runEVMIR([While(cond, Block(i))], s, k) ==
+    //         runEVM(
+    //             1,
+    //             toEVM(While(cond, Block(i))),
+    //             s, 
+    //             n).0
+    // {
+    //     //  For convenience and clarity, store program in a var 
+    //     var p :=  toEVM(While(cond, Block(i)));
+    //     if n < 2 {
+    //         //  Only one step can be simulated so the instruction at pc is not executed.
+    //         k := 0;
+    //     } else if n < 3 {
+    //         //  Exactly two steps in the EVM. 
+    //         assert n == 2;
+    //         if cond(s) {
+    //             k := 1;
+    //         } else {
+    //             assert !cond(s);
+    //             k := 0;
+    //         }
+    //     } else {
+    //         //  More than 2 steps in the EVM. So at least one iteration of the EVM body.
+    //         assert n > 2;
+    //         if cond(s) {
+    //             calc == {
+    //                 runEVM(1, p, s, n);
+    //                 runEVM(2, p, s, n - 1);
+    //                 runEVM(3, p, runInst(i, s), n - 2);
+    //                 runEVM(1, p, runInst(i, s), n - 3);
+    //             }
+    //             //  Because body of while and jump progs are the same, they reach the same
+    //             //  state after one iteration of the body.
+    //             calc == {
+    //                 runEVMIR([While(cond, Block(i))], s, n);
+    //                 runEVMIR([While(cond, Block(i))], runInst(i, s), n - 1);
+    //             }
+    //             //  And by induction, we can get a simulation for the n - 3 remaining steps compute the same
+    //             //  result.
+    //             var xk := singleWhileSim(i, cond, n - 3, runInst(i, s));
+    //             //  Overall we do the body of the loop once and then in xk steps simulate the rest.
+    //             k := 1 + xk;
+    //         } else {
+    //             //  Exit the loop.
+    //             assert !cond(s);
+    //             k := 1;
+    //         }    
+    //     }
+    // }    
         
+    /**
+     *  If Then Else Simulation proof. Assume unique block in ifBody and ifElse.
+     *
+     *  @returns    The (minimum) number of steps in the EVMIR to simulate n steps in EVM. 
+     */
+    lemma ifTheElseSim<S>(i1: EVMInst, i2: EVMInst, cond: S -> bool, n: nat, s: S) returns (k: nat)
+        requires n > 2
+        ensures k <= n && runEVMIR([IfElse(cond, Block(i1), Block(i2))], s, k) ==  
+            runEVM2(
+                0,
+                toEVM(IfElse(cond, Block(i1), Block(i2))),
+                s, 
+                n).0
+    { 
+        var p := toEVM(IfElse(cond, Block(i1), Block(i2)));
+        if n < 3 {
+            //  if less than 1 step, only evaluate condition which takes no steps in EVM-IR
+            if n <= 1 {
+                k := 0 ;
+            } else {
+                //  Evaluate condition and execute i1 or i2. One step in EVM-IR
+                k := 1;
+            }
+        } else {
+            if cond(s) {
+                //  Execute the ifBody
+                calc == {
+                    runEVM2(0, p, s, n);
+                    runEVM2(1, p, s, n - 1);
+                    runEVM2(2, p, runInst(i1, s), n - 2);
+                    runEVM2(4, p, runInst(i1, s), n - 3);
+                }
+                //  EVM-IR program simulates p in 2 steps
+                calc == {
+                    runEVMIR([IfElse(cond, Block(i1), Block(i2))], s, n);
+                    runEVMIR([], runInst(i1, s), n - 1);
+                    runInst(i1, s);
+                }
+                k := n - 2;
+            } else {
+                assert !cond(s);
+                calc == {
+                    runEVM2(0, p, s, n);
+                    runEVM2(3, p, s, n - 1);
+                    runEVM2(4, p, runInst(i2, s), n - 2);
+                }
+                //  EVM-IR program simulates p in 2 steps
+                calc == {
+                    runEVMIR([IfElse(cond, Block(i1), Block(i2))], s, n);
+                    runEVMIR([], runInst(i2, s), n - 1);
+                    runInst(i2, s);
+                }
+                k := n - 2;
+            }
+        }
+    }
+
 
 }
